intermediate step

compiler/proof_vec/equiv_poly1305_avx.ec
@@ -1,21 +1,5 @@
 require import AllCore IntDiv List CoreMap Jasmin_model.
-require import Poly1305_amd64_5x Poly1305_avx_5x Poly1305_avx_5xp.
-
-hint simplify pow_le0.
-hint simplify powS_minus@1.
-hint simplify
-  (pow2_1, pow2_2, pow2_3, pow2_4, pow2_5, pow2_6, pow2_7, pow2_8)@0.
-
-lemma pow2_32 : 2 ^ 32 = 4294967296.
-proof. by cbv delta. qed.
-
-lemma pow2_64 : 2 ^ 64 = 18446744073709551616.
-proof. by cbv delta. qed.
-
-lemma pow2_128 : 2 ^ 128 = 340282366920938463463374607431768211456.
-proof. by cbv delta. qed.
-
-hint simplify (pow2_32, pow2_64, pow2_128)@0.
+require import Poly1305_amd64_5x Poly1305_amd64_5xPR Poly1305_avx_5x Poly1305_avx_5xp.
 
 axiom W128_unpack_2u64_of_uint i : 
   unpack_2u64 (W128.of_uint i) = 
@@ -29,8 +13,6 @@ axiom W64_unpack_2u32_of_uint i :
     let i = i %% (2^ W64.size) in
     (W32.of_uint (i %% 2^32), W32.of_uint (i %/ 2^32)).
   
-
-
 hint simplify W64_unpack_2u32_of_uint.
 
 hint simplify (pack_unpack_2u64, unpack_pack_2u64)@0.
@@ -54,7 +36,7 @@ hint simplify (Array10.get_set_eqE, Array10.get_set_neqE)@0.
 hint simplify (iota0, iotaS_minus)@0.
 
 (* ------------------------------------------------------------------------------ *)
-(* AVX and its optimized version                                                  *)
+(* AVX-5x and its optimized version AVX-5xp                                       *)
 (* ------------------------------------------------------------------------------ *)
 
 equiv poly1305_avx_5x_5xp : 
@@ -71,6 +53,54 @@ proof.
   swap{2} 51 6;sim.
 qed.
 
+(* ------------------------------------------------------------------------------ *)
+(* AMD64-5x and AMD64-5x_for_proof                                                *)
+(* ------------------------------------------------------------------------------ *)
+
+equiv amd64_amd64_pr_load : Poly1305_amd64_5x.M.load ~ Poly1305_amd64_5xPR.M.load :
+   ={global_mem, in_0} ==> ={res}.
+proof. sim. qed.
+
+equiv poly1305_amd64_amd64_pr : 
+  Poly1305_amd64_5x.M.poly1305 ~ Poly1305_amd64_5xPR.M.poly1305 :
+    ={arg} ==> ={res}.
+proof.
+  proc => /=; sim (_:true).
+  + proc.    
+    swap{1} 10 2.
+    swap{1} [12..15] 2.
+    swap{1} 17 5. swap{1} 18 -4. swap{1} 21 -6.
+    swap{1} 18 2. swap{1} 18 -1.
+    swap{2} [10..11] -1.
+    inline{2} Poly1305_amd64_5xPR.M.unpack_u128x2_to_u26x5x2
+              Poly1305_amd64_5xPR.M.mulmod_u128
+              Poly1305_amd64_5xPR.M.add_u128
+              Poly1305_amd64_5xPR.M.carry_reduce_u128.
+    sim; wp.
+    call amd64_amd64_pr_load;wp => /=.
+    seq 7 6 : (#pre); 1:by sim.
+    conseq />.
+    transitivity{1} {
+      x0 <@ Poly1305_amd64_5x.M.load(global_mem, in_0);
+      x1 <@ Poly1305_amd64_5x.M.load(global_mem, in_0 + (of_uint 32)%W64);
+      y0 <@ Poly1305_amd64_5x.M.load(global_mem, in_0 + (of_uint 32)%W64 - (of_uint 16)%W64);
+      in_0 <- in_0 + (of_uint 32)%W64 - (of_uint 16)%W64;
+    } 
+      (={global_mem, in_0, s_r2, s_r2x5} ==> ={global_mem, in_0, x0, x1, y0})
+      (={global_mem, in_0, s_r2, s_r2x5} ==> (global_mem{2} = global_mem1{2} /\
+             in_0{1} + (of_uint 32)%W64 = in_01{2} + (of_uint 16)%W64) /\
+             (in_0{1} + (of_uint 32)%W64 = in_01{2} + (of_uint 16)%W64 =>
+             in_0{1} + (of_uint 32)%W64 + (of_uint 16)%W64 = in_0{2} + (of_uint 32)%W64 /\
+             ={y0} /\ x1{1} = x2{2} /\ ={x0}))=> //.
+    + by move=> &m1 &m2 />; exists global_mem{m2} in_0{m2} s_r2{m2} s_r2x5{m2}.
+    + do !(wp;call (_: ={global_mem, in_0} ==> ={res}); 1: by sim).
+     
+amd64_amd64_pr_load.
+
+#post).
+
+    sp.
+in_0{1} 
 (* ------------------------------------------------------------------------------ *)
 (* AMD64-5x and AVX-5x                                                            *)
 (* ------------------------------------------------------------------------------ *)
@@ -90,75 +120,95 @@ op rela5 (x y: W64.t Array5.t)
   xy.[3] = pack_2u64 (x.[3], y.[3]) /\
   xy.[4] = pack_2u64 (x.[4], y.[4]).
 
-op is_x5 (z zx5 : W64.t Array5.t) = 
+op is_x5 (z : W64.t Array5.t) (zx5 : W64.t Array4.t) = 
   zx5.[0] = z.[1] * W64.of_uint 5 /\
   zx5.[1] = z.[2] * W64.of_uint 5 /\
   zx5.[2] = z.[3] * W64.of_uint 5 /\
   zx5.[3] = z.[4] * W64.of_uint 5.
 
-phoare unpack_u26x5x2P x0 y0:
-   [Poly1305_avx_5x.M.unpack_u26x5x2_to_u26x5x2 :
-    s = x0 /\ t = y0 ==> rela5 x0 y0 res] = 1%r.
+op bounded n (w:W64.t) = 
+  W64.to_uint w < 2^n
+  axiomatized by boundedE.
+
+op wf5 (z : W64.t Array5.t) = 
+   bounded 27 z.[0] /\
+   bounded 27 z.[1] /\
+   bounded 27 z.[2] /\
+   bounded 27 z.[3] /\
+   bounded 27 z.[4].
+
+op wf4 (z : W64.t Array4.t) = 
+   bounded 31 z.[0] /\
+   bounded 31 z.[1] /\
+   bounded 31 z.[2] /\
+   bounded 31 z.[3].
+
+axiom bounded_add i x y : 0 < i => bounded (i-1) x => bounded (i-1) y => bounded i (x + y).
+axiom bounded_and i x y : bounded i x \/ bounded i y => bounded i (x `&` y).
+axiom bounded_shr i j x : 
+  0 <= i => (* i + j <= 64 => *)
+  bounded (i + j) x => 
+  bounded i (x `>>` W8.of_uint j).
+axiom bounded_mul i j x y:
+  bounded i x => 
+  bounded j y =>
+  bounded (i+j) (x * y).
+
+axiom bounded_weak (i j:int) x : i <= j => bounded i x => bounded j x.
+
+axiom bounded_w64 i w : 64 <= i => bounded i w.
+
+(*lemma bounded_5 i : 4 <= i => bounded i (W64.of_uint 5).
+proof. by move=> ?;apply (bounded_weak 4). qed.
+
+lemma bounded_67108863 i : 26 <= i => bounded 26 (W64.of_uint 67108863).
+proof. by move=> ?;apply (bounded_weak 26). qed. *)
+
+lemma bounded_and_2p26 i w : 26 <= i => bounded i (w `&`  (W64.of_uint 67108863)).
 proof.
-  proc.
-  (* FIXME "unroll for 3", should work *)
-  unroll 3; rcondt 3; 1: by auto.
-  unroll 7; rcondt 7; 1: by auto.
-  unroll 11; rcondt 11; 1: by auto.
-  unroll 15; rcondt 15; 1: by auto.
-  unroll 19; rcondt 19; 1: by auto.
-  rcondf 23; 1: by auto.
-  wp;skip;cbv delta => />.
+  move=> h; apply (bounded_weak 26); 1: done.
+  by apply bounded_and;right;rewrite boundedE. 
 qed.
 
-op bounded_32 (w:W64.t) = W64.to_uint w < 2^32.
-
-op bounded_32_5 (z: W64.t Array5.t) = 
-  bounded_32 z.[0] /\
-  bounded_32 z.[1] /\
-  bounded_32 z.[2] /\
-  bounded_32 z.[3] /\
-  bounded_32 z.[4].
-
-(* axiom to_uint_pos w : 0 <= W64.to_uint w. *)
-axiom to_uint_LAND_r (w1 w2:W64.t) : W64.to_uint (w1 `&` w2) <= W64.to_uint w2.
-
-import StdOrder.IntOrder.
-
-lemma bounded_32_LAND_r (w1 w2:W64.t) : W64.to_uint w2 < 2^32 => bounded_32 (w1 `&` w2).
+lemma bounded_mul5 i w : bounded (i-4) w => bounded i (w * (W64.of_uint 5)).
 proof.
-  rewrite /bounded_32 => h. 
-  apply (ler_lt_trans (to_uint w2)) => //.
-  by apply to_uint_LAND_r.
+  move=> h; have -> : i = (i - 4) + 4 by ring.
+  by apply bounded_mul => //; rewrite boundedE.
+qed.
+
+hoare carry_reduceWF : Poly1305_amd64_5x.M.carry_reduce : true ==> wf5 res.
+proof.
+  proc; wp; skip; rewrite /wf5 => &m1 &m2 /=.
+  smt (bounded_and_2p26 bounded_add bounded_shr bounded_mul5 bounded_w64).
 qed.
 
 equiv carry_reduceP : Poly1305_amd64_5x.M.carry_reduce ~ Poly1305_avx_5x.M.carry_reduce : 
-        ={x} ==> ={res} /\ bounded_32_5 res{1}.
+        ={x} ==> ={res} /\ wf5 res{1}.
 proof.
-  proc; wp; skip; rewrite /bounded_32_5 => &m1 &m2 /= -> /=.
-  split; 1: by apply bounded_32_LAND_r; cbv delta.
-  split.
-  + admit.
-  split; 1: by apply bounded_32_LAND_r; cbv delta.
-  split; 1: by apply bounded_32_LAND_r; cbv delta.
-  admit.
-admitted.
+  conseq (_: ={res}) carry_reduceWF.
+  by proc; wp; skip => &m1 &m2 /= ->.
+qed.
+
+hoare clampWF : Poly1305_amd64_5x.M.clamp : true ==> wf5 res.
+proof.
+  proc;wp; conseq (_:true);last done.
+  rewrite /wf5 /= => ?.
+  do !(split || by apply bounded_and;right;rewrite boundedE).
+qed.
 
 equiv clampP : Poly1305_amd64_5x.M.clamp ~ Poly1305_avx_5x.M.clamp : 
-  ={global_mem, k} ==> ={res} /\ bounded_32_5 res{1}.
+  ={global_mem, k} ==> ={res} /\ wf5 res{1}.
 proof.
-  proc.
-  seq 2 2 : (={r}); 1: by sim.
-  auto; rewrite /bounded_32_5 /= => ?? -> /=.
-  by rewrite !bounded_32_LAND_r; cbv delta.
+  conseq (_: ={res}) clampWF.
+  proc; sim.
 qed.
-  
+
 axiom pack_mulu_32 w1 w2 : 
   pack_2u32 (W32.mulu w1 w2) = (zeroext_32_64 w1) * (zeroext_32_64 w2).
 
 hint simplify pack_mulu_32.
 
-axiom zeroext_bounded w : bounded_32 w => zeroext_32_64 (unpack_2u32 w).`1 = w.
+axiom zeroext_bounded w : bounded 32 w => zeroext_32_64 (unpack_2u32 w).`1 = w.
 
 lemma zeroext_of_uint i : zeroext_32_64 (W32.of_uint i) = W64.of_uint (i %% W32.modulus).
 proof. by rewrite zeroext_32_64E. qed.
@@ -183,11 +233,10 @@ proof.
   call (add_carryP) => /=.
   conseq (_: Array5.all_eq x{1} h{2} /\ Array5.all_eq y{1} t{2}).
   + by move=> ?????;rewrite !Array5.ext_eq_all.
-  unroll for {2} 5; wp; skip => &m1 &m2; cbv delta => [#] 5!-> /=.
-  admit. (* We need to have a symmetry in the code *)
+  by unroll for {2} 5; wp; skip => &m1 &m2; cbv delta => [#] 5!->.
 qed.
 
-hint simplify (VPAND_128_64, VPOR_128_64, VPXOR_128_64)@0.
+hint simplify (VPAND_128_64, VPOR_128_64, VPXOR_128_64)@0. 
 
 lemma VPAND_128_64_l w1 w2 : 
    pack_2u64 w1 `&` w2 = 
@@ -197,6 +246,7 @@ proof. by rewrite -(pack_unpack_2u64 w2) VPAND_128_64. qed.
 hint simplify VPAND_128_64_l@1.
 
 equiv final_mulP : Poly1305_amd64_5x.M.final_mul ~ Poly1305_avx_5x.M.final_mul : 
+  wf5 hx{1} /\ wf5 hy{1} /\ wf5 s_r2{1} /\ wf4 s_r2x5{1} /\ wf5 s_r{1} /\ wf4 s_rx5{1} /\
   rela5 hx{1} hy{1} hxy{2} /\
   rela5 s_r2{1} s_r{1} s_r2r{2} /\
   rela4 s_r2x5{1} s_rx5{1} s_r2rx5{2} ==> ={res}.
@@ -205,11 +255,64 @@ proof.
   call hadd_u128P => /=.
   swap{1} 7 3. swap{1} 6 2. swap{1} 6 -1; wp.
   seq 7 2 : (#post).   
-  + inline *; wp; skip. cbv delta.
-    move=> &m1 &m2 [#] 14!-> />.
+  + inline *; wp; skip; cbv delta.
+    move=> &m1 &m2 [#] X0 X1 X2 X3 X4 Y0 Y1 Y2 Y3 Y4.
+    move=> R20 R21 R22 R23 R24 R2x0 R2x1 R2x2 R2x3.
+    move=> R0 R1 R2 R3 R4 Rx0 Rx1 Rx2 Rx3 14!-> />.
+    rewrite (zeroext_bounded hx{m1}.[0]). by move: X0;apply: bounded_weak.
+    rewrite (zeroext_bounded hx{m1}.[1]). by move: X1;apply: bounded_weak.
+    rewrite (zeroext_bounded hx{m1}.[2]). by move: X2;apply: bounded_weak.
+    rewrite (zeroext_bounded hx{m1}.[3]). by move: X3;apply: bounded_weak.
+    rewrite (zeroext_bounded hx{m1}.[4]). by move: X4;apply: bounded_weak.
+    rewrite (zeroext_bounded hy{m1}.[0]). by move: Y0;apply: bounded_weak.
+    rewrite (zeroext_bounded hy{m1}.[1]). by move: Y1;apply: bounded_weak.
+    rewrite (zeroext_bounded hy{m1}.[2]). by move: Y2;apply: bounded_weak.
+    rewrite (zeroext_bounded hy{m1}.[3]). by move: Y3;apply: bounded_weak.
+    rewrite (zeroext_bounded hy{m1}.[4]). by move: Y4;apply: bounded_weak.
+    rewrite (zeroext_bounded s_r2{m1}.[0]). by move: R20;apply: bounded_weak.
+    rewrite (zeroext_bounded s_r2{m1}.[1]). by move: R21;apply: bounded_weak.
+    rewrite (zeroext_bounded s_r2{m1}.[2]). by move: R22;apply: bounded_weak.
+    rewrite (zeroext_bounded s_r2{m1}.[3]). by move: R23;apply: bounded_weak.
+    rewrite (zeroext_bounded s_r2{m1}.[4]). by move: R24;apply: bounded_weak.
+    rewrite (zeroext_bounded s_r2x5{m1}.[0]). by move: R2x0;apply: bounded_weak.
+    rewrite (zeroext_bounded s_r2x5{m1}.[1]). by move: R2x1;apply: bounded_weak.
+    rewrite (zeroext_bounded s_r2x5{m1}.[2]). by move: R2x2;apply: bounded_weak.
+    rewrite (zeroext_bounded s_r2x5{m1}.[3]). by move: R2x3;apply: bounded_weak.
+    rewrite (zeroext_bounded s_r{m1}.[0]). by move: R0;apply: bounded_weak.
+    rewrite (zeroext_bounded s_r{m1}.[1]). by move: R1;apply: bounded_weak.
+    rewrite (zeroext_bounded s_r{m1}.[2]). by move: R2;apply: bounded_weak.
+    rewrite (zeroext_bounded s_r{m1}.[3]). by move: R3;apply: bounded_weak.
+    rewrite (zeroext_bounded s_r{m1}.[4]). by move: R4;apply: bounded_weak.
+    rewrite (zeroext_bounded s_rx5{m1}.[0]). by move: Rx0;apply: bounded_weak.
+    rewrite (zeroext_bounded s_rx5{m1}.[1]). by move: Rx1;apply: bounded_weak.
+    rewrite (zeroext_bounded s_rx5{m1}.[2]). by move: Rx2;apply: bounded_weak.
+    rewrite (zeroext_bounded s_rx5{m1}.[3]). by move: Rx3;apply: bounded_weak.
+    done.
+
+
+
+ X0.
+s_r2{m2}.[1])
+    rewrite !zeroext_bounded. 
+    admit.
   inline *.
   wp; skip; cbv delta => &m1 &m2 [#] 5!->; cbv delta.
   admit. (* again we need condition on size *)
+qed.
+
+phoare unpack_u26x5x2P x0 y0:
+   [Poly1305_avx_5x.M.unpack_u26x5x2_to_u26x5x2 :
+    s = x0 /\ t = y0 ==> rela5 x0 y0 res] = 1%r.
+proof.
+  proc.
+  (* FIXME "unroll for 3", should work *)
+  unroll 3; rcondt 3; 1: by auto.
+  unroll 7; rcondt 7; 1: by auto.
+  unroll 11; rcondt 11; 1: by auto.
+  unroll 15; rcondt 15; 1: by auto.
+  unroll 19; rcondt 19; 1: by auto.
+  rcondf 23; 1: by auto.
+  wp;skip;cbv delta => />.
 qed.
 
 equiv remaining_blocksP : Poly1305_amd64_5x.M.remaining_blocks ~ Poly1305_avx_5x.M.remaining_blocks :
@@ -237,7 +340,15 @@ equiv first_blockP : Poly1305_amd64_5x.M.first_block ~ Poly1305_avx_5x.M.first_b
    rela5 res{1}.`1 res{1}.`2 res{2}.`1.
 admitted.
 
-axiom W64_leNgt (w1 w2: W64.t) : (w1 `<=` w2) = ! (w2 `<` w1).
+(* axiom W64_leNgt (w1 w2: W64.t) : (w1 `<=` w2) = ! (w2 `<` w1). *)
+
+
+unpack 26 26 26 26 24
+r4 : 26 26 26 26 24
+r4x5 : 30 30 30 28
+
+mulmod 56 
+61       
 
 equiv poly1305_amd64_avx_5x :
   Poly1305_amd64_5x.M.poly1305 ~ Poly1305_avx_5x.M.poly1305 :
